experiment/Experiment.Steel.Monad.Test.fst
@@ -34,28 +34,6 @@ open Experiment.Steel
 
 #push-options "--ide_id_info_off"
 
-(* TODO: LV -> SF is long
-   TODO: MV
- *)
-inline_for_extraction
-let test_par0 (r0 r1 : ref U32.t)
-  : F.usteel unit (vptr r0 `star` vptr r1) (fun _ -> vptr r0 `star` vptr r1)
-      (requires fun _ -> True) (ensures fun _ _ h1 -> sel r0 h1 = 0ul /\ sel r1 h1 = 0ul)
-  = F.(to_steel #[Timer; Dump Stage_WP] (
-    _ <-- GCb.par (vptr r0) (vptr r1)
-      (call (write r0) 0ul)
-      (call (write r1) 0ul);
-    return ()
-  ) ())
-// time specs     : 101ms
-// time lin_cond  : 631ms
-// time sub_push  : 124ms
-// time LV2SF     : 7362ms
-// time SF2Fun    : 3ms
-// time Fun_wp    : 586ms
-// total time : 8807ms
-
-
 irreducible let __test__ : unit = ()
 let norm_test () = T.norm [delta_qualifier ["unfold"]; delta_attr [`%__test__]]
 
@@ -647,3 +625,22 @@ let test_for_loop_1 (r0 r1 : ref U32.t)
 // memory to finish processing the definition.
 // The term resulting from the normalisation is quite big because of the (ghost) tree_cond
 // used for the specifications on our Steel combinators.
+
+
+inline_for_extraction
+let test_par0 (r0 r1 : ref U32.t)
+  : F.usteel unit (vptr r0 `star` vptr r1) (fun _ -> vptr r0 `star` vptr r1)
+      (requires fun _ -> True) (ensures fun _ _ h1 -> sel r0 h1 = 0ul /\ sel r1 h1 = 0ul)
+  = F.(to_steel #[Timer; Dump Stage_WP] (
+    _ <-- GCb.par (vptr r0) (vptr r1)
+      (call (write r0) 0ul)
+      (call (write r1) 0ul);
+    return ()
+  ) ())
+// time specs     : 86ms
+// time lin_cond  : 870ms
+// time sub_push  : 179ms
+// time LV2SF     : 6955ms
+// time SF2Fun    : 3ms
+// time Fun_wp    : 428ms
+// total time : 8521ms
